rocq-bluerock-brick/theories/lang/cpp/logic/pred2.v
@@ -1,0 +1,1556 @@
+(*
+ * Copyright (c) 2020-2023 BlueRock Security, Inc.
+ * This software is distributed under the terms of the BedRock Open-Source License.
+ * See the LICENSE-BedRock file in the repository root for details.
+ *)
+(** This file defines the core logic (called [mpred]) that we use
+    for C++.
+
+    Known issues:
+    - currently the logic is sequentially consistent
+    - the memory model is simplified from the standard C++ memory
+      model.
+ *)
+Require Import elpi.apps.locker.locker.
+Require Export bedrock.prelude.addr.
+
+Require Export bedrock.lang.bi.prelude.
+Require Export bedrock.lang.bi.observe.
+Require Export bedrock.lang.bi.spec.knowledge.
+Require Export bedrock.lang.cpp.reserved_notation.
+Require Export bedrock.lang.cpp.logic.mpred.
+Require Export bedrock.lang.cpp.logic.rep.
+(** ^^ Delicate; export types and canonical structures (CS) for [monPred], [mpred] and [Rep].
+Export order can affect CS inference. *)
+
+Require Import bedrock.prelude.bytestring.
+
+Require Export bedrock.lang.cpp.algebra.cfrac.
+Require Export bedrock.lang.cpp.bi.cfractional.
+
+Require Export iris.base_logic.lib.iprop.
+(* TODO: ^^ only needed to export uPredI, should be removed. *)
+Require Import iris.bi.lib.fractional.
+Require Import bedrock.lang.proofmode.proofmode.
+
+Require Import bedrock.lang.bi.na_invariants.
+Require Import bedrock.lang.bi.cancelable_invariants.
+Export ChargeNotation.
+Require Import bedrock.lang.cpp.bi.cfractional.
+
+Require Import bedrock.lang.cpp.syntax.
+Require Import bedrock.lang.cpp.semantics.values2.
+Require Import bedrock.lang.cpp.semantics.subtyping.
+Require Import bedrock.lang.cpp.semantics.ptrs2.
+
+#[local] Set Printing Coercions.
+
+Variant validity_type : Set := Strict | Relaxed.
+
+Implicit Types (vt : validity_type) (σ resolve : genv).
+Implicit Types (n : N) (z : Z).
+
+(* Namespace for the invariants of the C++ abstraction's ghost state. *)
+Definition pred_ns : namespace := nroot .@@ "bedrock" .@@ "lang" .@@ "cpp_logic".
+
+(* Used by [has_type_prop_has_type_noptr]. No theory. *)
+Definition nonptr_prim_type {lang} (ty : type' lang) : bool :=
+  match drop_qualifiers ty with
+  | Tfloat_ _ | Tchar_ _ | Tvoid | Tbool | Tenum _ | Tnum _ _ => true
+  | Tnullptr | Tptr _ | Tref _ | Trv_ref _ | _ => false
+  end.
+
+Lemma nonptr_prim_type_erase_qualifiers : forall {lang} (ty : type' lang),
+    nonptr_prim_type ty = nonptr_prim_type (erase_qualifiers ty).
+Proof. induction ty; simpl; eauto. Qed.
+
+Module Type CPP_LOGIC
+  (Import P : PTRS_INTF)
+  (Import INTF : VALUES_INTF_FUNCTOR P)
+  (Import CC : CPP_LOGIC_CLASS).
+
+  Implicit Types (p : ptr).
+
+  Section with_cpp.
+
+    (**
+      [_valid_ptr vt p] is a persistent assertion that [p] is a _valid pointer_, that is:
+      - [p] can point to a function or a (possibly dead) object [o]
+      - if [vt = Relaxed], [p] can be nullptr, or past-the-end of a (possibly dead) object [o].
+      In particular, [_valid_ptr vt p] prevents producing [p] by incrementing
+      past-the-end pointers into overflow territory.
+
+      Our definition of validity includes all cases in which a pointer is not
+      an _invalid pointer value_ in the sense of the standard
+      (<https://eel.is/c++draft/basic.compound#3.1>), except that our concept
+      of validity survives deallocation; a pointer is only valid according to
+      the standard (or "standard-valid") if it is _both_ valid ([_valid_ptr
+      vt p]) and live ([live_ptr p]); we require both where needed (e.g.
+      [eval_ptr_eq]).
+
+      When the duration of a region of storage ends [note 1], contained objects [o] go
+      from live to dead, and pointers to such objects become _dangling_, or
+      _invalid pointer values_ (<https://eel.is/c++draft/basic.compound#3.1>);
+      this is called _pointer zapping_ [note 1].
+      In our semantics, that only consumes the non-persistent predicate
+      [live_ptr p], not the persistent predicate [_valid_ptr vt p].
+
+      Following Cerberus, [live_alloc_id] tracks liveness per allocation
+      ID (see comments for [ptr]), and [live_ptr] is derived from it. Hence,
+      a pointer [p] past-the-end of [o] also becomes dangling when [o] is
+      deallocated.
+
+      It's implementation-defined whether invalid pointer values are
+      (non-copyable) trap representations. Instead, we restrict to
+      implementations where dangling pointers are not trap representations
+      (which is allowed, since this choice is implementation-defined) and
+      pointer zapping does not actually clear pointers.
+
+      [Note 1]. See https://eel.is/c++draft/basic.stc.general#4 and
+      https://eel.is/c++draft/basic.compound#3.1 for C++, and
+      http://www.open-std.org/jtc1/sc22/wg14/www/docs/n2369.pdf for
+      discussion in the context of the C standard.
+    *)
+    Parameter _valid_ptr : forall `{!cpp_logic thread_info Σ}
+      (vt : validity_type), ptr -> mpred.
+    (* strict validity (not past-the-end) *)
+    Notation strict_valid_ptr := (_valid_ptr Strict).
+    (* validity (past-the-end allowed) *)
+    Notation valid_ptr := (_valid_ptr Relaxed).
+
+  Section with_cpp_logic.
+  Context `{cpp_logic}.
+
+    Axiom _valid_ptr_persistent : forall b p, Persistent (_valid_ptr b p).
+    Axiom _valid_ptr_affine : forall b p, Affine (_valid_ptr b p).
+    Axiom _valid_ptr_timeless : forall b p, Timeless (_valid_ptr b p).
+    #[global] Existing Instances _valid_ptr_persistent _valid_ptr_affine _valid_ptr_timeless.
+
+    Axiom valid_ptr_nullptr : |-- valid_ptr nullptr.
+    Axiom not_strictly_valid_ptr_nullptr : strict_valid_ptr nullptr |-- False.
+    Axiom strict_valid_valid : forall p,
+      strict_valid_ptr p |-- valid_ptr p.
+
+  End with_cpp_logic.
+
+    (**
+    [has_type v ty] is an approximation in [mpred] of "[v] is an initialized value
+    of type [t]." This is intended to be preserved by the C++ type system.
+    TODO: include in [primR].
+    TODO: refine for which types https://bedrocksystems.atlassian.net/browse/FM-3760
+    *)
+    Parameter has_type : ∀ `{!cpp_logic thread_info Σ} {σ : genv}, val -> type -> mpred.
+
+    #[global] Declare Instance has_type_mono `{cpp_logic} :
+      Proper (genv_leq ==> eq ==> eq ==> (⊢)) (@has_type _ _ _).
+
+    (**
+       [reference_to ty p] states that the location [p] stores a value of type [ty].
+       Being a reference is stronger than being a pointer because pointers allow
+       past-the-end pointers while references do not.
+
+       This should be thought of as closely related to [has_type (Vref p) (Tref ty)]
+       except that it holds on types that are not valid C++ types. For example,
+       if
+       <<
+       struct C { int& r; } x;
+       >>
+       then [reference_to (Tref Tint) (x ., ``::C::r``)].
+
+       In the future, [has_type (Vref (x ., ``::C::r``)) (Tref (Tref Tint))]
+       may not hold since [Tref (Tref Tint)] is not a valid C++ type. The
+       current blocker to this is that we use [tptsto] to represent
+       ownership of references. This would need to change.
+
+       Note that the following code is (currently?) legal according to our
+       semantics:
+       <<
+       { long x; *static_cast<int*>(&x); }
+       >>
+       because [reference_to] only guarantees alignment, not anything
+       about the dynamic type of the object. Requiring a property of the dynamic
+       type of the object would require us to carry type information in
+       [strict_valid_ptr] (which would make it something like a pre-construction
+       state of [type_ptr]).
+     *)
+    Parameter reference_to : forall `{!cpp_logic thread_info Σ} {σ : genv}, type -> ptr -> mpred.
+
+    #[global] Declare Instance reference_to_mono `{cpp_logic} :
+      Proper (genv_leq ==> eq ==> eq ==> (⊢)) (@reference_to _ _ _).
+
+    Section with_genv.
+      Context `{cpp_logic} {σ : genv}.
+
+      #[global] Declare Instance has_type_knowledge : Knowledge2 has_type.
+      #[global] Declare Instance has_type_timeless : Timeless2 has_type.
+
+      Axiom has_type_has_type_prop : ∀ v ty, has_type v ty |-- [| has_type_prop v ty |].
+
+      Axiom has_type_prop_has_type_noptr : ∀ v ty,
+        nonptr_prim_type ty ->
+        [| has_type_prop v ty |] |-- has_type v ty.
+
+      (* [has_type] is independent of qualifiers.
+         This allows casting betweeen [const] and non-[const].
+         *)
+      Axiom has_type_erase_qualifiers : ∀ ty v,
+        has_type v ty -|- has_type v (erase_qualifiers ty).
+
+      (* Internal statements: *)
+      Axiom has_type_nullptr' : ∀ p,
+        has_type (Vptr p) Tnullptr -|- [| p = nullptr |].
+      Axiom has_type_ptr' : ∀ p ty,
+        has_type (Vptr p) (Tptr ty) -|-
+        valid_ptr p ** [| aligned_ptr_ty ty p |].
+
+      (* These two definitions are needed because of [tptsto_has_type] *)
+      Axiom has_type_ref' : ∀ p ty,
+        has_type (Vref p) (Tref ty) |-- reference_to ty p.
+      Axiom has_type_rv_ref' : ∀ p ty,
+        has_type (Vref p) (Trv_ref ty) |-- reference_to ty p.
+
+      #[global] Declare Instance reference_to_knowledge : Knowledge2 reference_to.
+      #[global] Declare Instance reference_to_timeless : Timeless2 reference_to.
+
+      (* NOTE: this is almost derivable from [reference_to_intro] and
+         [reference_to_elim] except for the issue with non-standard types. *)
+      Axiom reference_to_erase : forall ty p,
+          reference_to ty p -|- reference_to (erase_qualifiers ty) p.
+
+      (** The introduction and elimination forms are not the same
+          to avoid using [has_type] as types that are not C++ types.
+          In practice, the only way to prove a [reference_to] is to have
+          a [tptsto] assertion.
+
+          **A note on 0-sized objects**
+          0-sized objects are problematic from the point of view of C++ (they are not
+          permitted by the standard, but they are supported by standard compilers).
+          The problem with 0-sized objects is that they do not have a unique identity
+          but the BRiCk semantics will give them an identity using
+          [struct_padding]/[union_padding].
+
+          Mitigation: We currently address this by forbidding reasoning about
+                      constructors of 0-sized objects.
+       *)
+      Axiom reference_to_intro : forall ty p,
+          strict_valid_ptr p |-- has_type (Vptr p) (Tptr ty) -* reference_to ty p.
+      Axiom reference_to_elim : forall ty p,
+          reference_to ty p |--
+            [| aligned_ptr_ty ty p |] ** [| p <> nullptr |] **
+            valid_ptr p ** if zero_sized_array ty then emp else strict_valid_ptr p.
+
+    End with_genv.
+
+    Parameter has_type_or_undef : forall `{!cpp_logic thread_info Σ} {σ : genv}, val -> type -> mpred.
+    Axiom has_type_or_undef_unfold : forall `{cpp_logic},
+        @has_type_or_undef _ _ _ = funI σ v ty => has_type v ty \\// [| v = Vundef |].
+
+    (** Formalizes the notion of "provides storage",
+    http://eel.is/c++draft/intro.object#def:provides_storage *)
+    Parameter provides_storage :
+      forall `{!cpp_logic thread_info Σ} (storage : ptr) (object : ptr) (object_type : Rtype), mpred.
+
+  Section with_cpp_logic.
+  Context `{cpp_logic}.
+
+    Axiom provides_storage_persistent :
+      forall storage_ptr obj_ptr ty,
+      Persistent (provides_storage storage_ptr obj_ptr ty).
+    Axiom provides_storage_affine :
+      forall storage_ptr obj_ptr ty,
+      Affine (provides_storage storage_ptr obj_ptr ty).
+    Axiom provides_storage_timeless :
+      forall storage_ptr obj_ptr ty,
+      Timeless (provides_storage storage_ptr obj_ptr ty).
+    #[global] Existing Instances provides_storage_persistent provides_storage_affine provides_storage_timeless.
+
+  End with_cpp_logic.
+
+    (** *** Typed points-to predicate.
+    Fact [tptsto t q p v] asserts the following things:
+    1. Pointer [p] points to value [v].
+    2. We have fractional ownership [q] (in the separation logic sense).
+    3. Pointer [p] points to a memory location with C++ type [t].
+    However:
+    1. Value [v] need not be initialized.
+    2. Hence, [v] might not satisfy [has_type_prop t v].
+
+    [tptsto] is only used to represent memory cells that contain
+    values representable as a single [val]. This includes:
+    - value types (see [is_value_type]), and
+    - reference types. Note that all gl-values, i.e. x-values ([Trv_ref])
+      and l-values ([Tref]), are represented using [Tref].
+    These requirements justify the axiom [tptsto_valid_type].
+
+    We use this predicate both for pointers to actual memory and for pointers to
+    C++ locations that are not stored in memory (as an optimization).
+    *)
+    Parameter tptsto : forall `{!cpp_logic thread_info Σ} {σ:genv}
+      (t : Rtype) (q : cQp.t) (a : ptr) (v : val), mpred.
+
+  Section with_cpp_logic.
+  Context `{cpp_logic}.
+
+    #[global] Declare Instance tptsto_valid_type
+      : forall {σ:genv} (t : Rtype) (q : cQp.t) (a : ptr) (v : val),
+        Observe [| is_heap_type t |] (tptsto t q a v).
+
+    Axiom tptsto_nonnull : forall {σ} ty q a,
+      tptsto (σ:=σ) ty q nullptr a |-- False.
+
+    #[global] Declare Instance tptsto_params : Params (@tptsto) 3.
+    #[global] Declare Instance tptsto_proper :
+      Proper (genv_eq ==> eq ==> eq ==> eq ==> eq ==> (≡)) (@tptsto _ _ _).
+    #[global] Declare Instance tptsto_mono :
+      Proper (genv_leq ==> eq ==> eq ==> eq ==> eq ==> (⊢)) (@tptsto _ _ _).
+
+    #[global] Declare Instance tptsto_timeless : Timeless5 (@tptsto _ _ _).
+    #[global] Declare Instance tptsto_cfractional {σ} ty : CFractional2 (tptsto ty).
+
+    #[global] Declare Instance tptsto_cfrac_valid {σ} t : CFracValid2 (tptsto t).
+
+    #[global] Declare Instance tptsto_welltyped : forall {σ} p ty q v,
+      Observe (has_type_or_undef v ty) (tptsto ty q p v).
+
+    #[global] Declare Instance tptsto_reference_to : forall {σ} p ty q v,
+      Observe (reference_to ty p) (tptsto ty q p v).
+
+    (**
+    NOTE: We'll eventually need the stronger [tptsto_learn : ∀ {σ} ty
+    q1 q2 p v1 v2, <absorb> (tptsto ty q1 p v1) //\\ <absorb> (tptsto
+    ty q2 p v2) |-- [! v1 = v2 !]] but setting up the proof in
+    [simple_pred] now would be a bit of a digression.
+    *)
+    #[global] Declare Instance tptsto_agree : forall {σ} ty q1 q2 p v1 v2,
+      Observe2 [| v1 = v2 |]
+               (tptsto ty q1 p v1)
+               (tptsto ty q2 p v2).
+
+    End with_cpp_logic.
+
+    (** The allocation is alive. Neither persistent nor fractional.
+      See https://eel.is/c++draft/basic.stc.general#4 and
+      https://eel.is/c++draft/basic.compound#3.1.
+    *)
+    Parameter live_alloc_id : forall `{!cpp_logic thread_info Σ},
+      alloc_id -> mpred.
+
+  Section with_cpp_logic.
+  Context `{cpp_logic}.
+
+    Axiom live_alloc_id_timeless : forall aid, Timeless (live_alloc_id aid).
+    #[global] Existing Instance live_alloc_id_timeless.
+
+    Axiom valid_ptr_alloc_id : forall p,
+      valid_ptr p |-- [| is_Some (ptr_alloc_id p) |].
+
+    (** This pointer is from a live allocation; this does not imply
+    [_valid_ptr], because even overflowing offsets preserve the allocation ID.
+    *)
+    Definition live_ptr (p : ptr) :=
+      default False%I (live_alloc_id <$> ptr_alloc_id p).
+
+    (** We consider [nullptr] as live, following Krebbers, as a way to
+    simplify stating rules for pointer comparison. *)
+    Axiom nullptr_live : |-- live_ptr nullptr.
+
+    Axiom tptsto_live : forall {σ} ty (q : cQp.t) p v,
+      tptsto ty q p v |-- live_ptr p ** True.
+
+  End with_cpp_logic.
+
+    (** [mdc_path σ this mdc q p] state that [p] is a pointer to a (live)
+        object of type [this] that is part of an object that can be reached
+        using the *path* [mdc]. The ownership [mdc_path] is only exposed to
+        the program for an object of class <<C>> if <<C>> has <<virtual>>
+        methods (or base classes, which are not currently supported).
+        - if [mdc = []] then this object mdc_path is not initialized yet,
+          e.g. because its base classes are still being constructed.
+        - otherwise, [mdc] is the *path* from the most derived class to this
+          object. For example, suppose you have:
+          <<
+          struct A { virtual int f() { return 0; } };
+          struct B : public A { virtual int f() { return 1; } };
+          struct C : public A { };
+          struct D : public B, public C { };
+
+          int doA(A* a) { return a->f(); }
+          int test() {
+              D d;
+              return doA(static_cast<B*>(&d)) /* = 1 */
+                   + doA(static_cast<C*>(&d)) /* = 0 */;
+          }
+          >>
+          for a fully constructed object of type `D` (at pointer [d]), you would
+          have:
+          [[
+          mdc_path "::B" ["::D","::B"]      1 (d ., _base "::B") **
+          mdc_path "::A" ["::D","::B","::A"] 1 (d ,, _base "::B" ,, _base "::A") **
+          mdc_path "::A" ["::D","::C","::A"] 1 (d ,, _base "::C" ,, _base "::A")
+          ]]
+          in the partially constructed state, where "::D" has not yet been constructed
+          but the base classes have been, you have the following:
+          [[
+          mdc_path "::B" ["::B"]      1 (d ., _base "::B") **
+          mdc_path "::A" ["::B","::A"] 1 (d ,, _base "::B" ,, _base "::A") **
+          mdc_path "::A" ["::C","::A"] 1 (d ,, _base "::C" ,, _base "::A")
+          ]]
+          Note that you do not get [mdc_path "::D" [] 1 d] at this point, you
+          get [mdc_path "::D" ["::D"] 1 d] when you update all the other paths
+          (but not atomically).
+
+        [mdc_path] is primarily used to dispatch <<virtual>> function calls.
+        Compilers can use the ownership here to represent dynamic dispatch
+        tables.
+     *)
+    Parameter mdc_path : forall `{!cpp_logic thread_info Σ} {σ : genv}
+        (this : globname) (most_derived : list globname),
+        cQp.t -> ptr -> mpred.
+
+  Section with_cpp_logic.
+  Context `{cpp_logic}.
+    #[global] Declare Instance mdc_path_cfractional σ this mdc : CFractional1 (mdc_path this mdc).
+    #[global] Declare Instance mdc_path_cfrac_valid {σ} cls path : CFracValid1 (mdc_path cls path).
+    #[global] Declare Instance mdc_path_timeless {σ} : Timeless4 (mdc_path).
+    #[global] Declare Instance mdc_path_strict_valid {σ} this mdc q p : Observe (strict_valid_ptr p) (mdc_path this mdc q p).
+    #[global] Declare Instance mdc_path_agree {σ} cls1 cls2 q1 q2 p mdc1 mdc2 :
+      Observe2 [| mdc1 = mdc2 /\ cls1 = cls2 |] (mdc_path cls1 mdc1 q1 p) (mdc_path cls2 mdc2 q2 p).
+
+    (** this allows you to forget an object mdc_path, necessary for doing
+        placement [new] over an existing object.
+     *)
+    Axiom mdc_path_forget : forall σ mdc this p,
+        mdc_path (σ:=σ) this mdc (cQp.m 1) p |-- |={↑pred_ns}=> mdc_path (σ:=σ) this nil (cQp.m 1) p.
+
+  End with_cpp_logic.
+
+    (** the pointer points to the code
+
+      note that in the presence of code-loading, function calls will
+      require an extra side-condition that the code is loaded.
+     *)
+    Parameter code_at : forall `{!cpp_logic thread_info Σ},
+      genv -> translation_unit -> Func -> ptr -> mpred.
+    Parameter method_at : forall `{!cpp_logic thread_info Σ},
+      genv -> translation_unit -> Method -> ptr -> mpred.
+    Parameter ctor_at : forall `{!cpp_logic thread_info Σ},
+      genv -> translation_unit -> Ctor -> ptr -> mpred.
+    Parameter dtor_at : forall `{!cpp_logic thread_info Σ},
+      genv -> translation_unit -> Dtor -> ptr -> mpred.
+    #[global] Arguments code_at {_ _ _ σ} tu _ _.
+    #[global] Arguments method_at {_ _ _ σ} tu _ _.
+    #[global] Arguments ctor_at {_ _ _ σ} tu _ _.
+    #[global] Arguments dtor_at {_ _ _ σ} tu _ _.
+
+
+    Section with_genv.
+      Context `{cpp_logic} {σ : genv} (tu : translation_unit).
+      #[local] Notation code_at := (@code_at _ _ _ σ tu) (only parsing).
+      #[local] Notation method_at := (@method_at _ _ _ σ tu) (only parsing).
+      #[local] Notation ctor_at := (@ctor_at _ _ _ σ tu) (only parsing).
+      #[local] Notation dtor_at := (@dtor_at _ _ _ σ tu) (only parsing).
+
+      Axiom code_at_persistent : forall f p, Persistent (code_at f p).
+      Axiom code_at_affine : forall f p, Affine (code_at f p).
+      Axiom code_at_timeless : forall f p, Timeless (code_at f p).
+
+      Axiom method_at_persistent : forall f p, Persistent (method_at f p).
+      Axiom method_at_affine : forall f p, Affine (method_at f p).
+      Axiom method_at_timeless : forall f p, Timeless (method_at f p).
+
+      Axiom ctor_at_persistent : forall f p, Persistent (ctor_at f p).
+      Axiom ctor_at_affine : forall f p, Affine (ctor_at f p).
+      Axiom ctor_at_timeless : forall f p, Timeless (ctor_at f p).
+
+      Axiom dtor_at_persistent : forall f p, Persistent (dtor_at f p).
+      Axiom dtor_at_affine : forall f p, Affine (dtor_at f p).
+      Axiom dtor_at_timeless : forall f p, Timeless (dtor_at f p).
+
+      #[global] Existing Instances
+        code_at_persistent code_at_affine code_at_timeless
+        method_at_persistent method_at_affine method_at_timeless
+        ctor_at_persistent ctor_at_affine ctor_at_timeless
+        dtor_at_persistent dtor_at_affine dtor_at_timeless.
+
+      Axiom code_at_live   : forall f p,   code_at f p |-- live_ptr p.
+      Axiom method_at_live : forall f p, method_at f p |-- live_ptr p.
+      Axiom ctor_at_live   : forall f p,   ctor_at f p |-- live_ptr p.
+      Axiom dtor_at_live   : forall f p,   dtor_at f p |-- live_ptr p.
+
+      Axiom code_at_strict_valid   : forall f p,   code_at f p |-- strict_valid_ptr p.
+      Axiom method_at_strict_valid : forall f p, method_at f p |-- strict_valid_ptr p.
+      Axiom ctor_at_strict_valid   : forall f p,   ctor_at f p |-- strict_valid_ptr p.
+      Axiom dtor_at_strict_valid   : forall f p,   dtor_at f p |-- strict_valid_ptr p.
+
+    End with_genv.
+
+  Section with_cpp_logic.
+  Context `{cpp_logic}.
+
+    Axiom offset_pinned_ptr_pure : forall σ o z va p,
+      eval_offset σ o = Some z ->
+      ptr_vaddr p = Some va ->
+      valid_ptr (p ,, o) |--
+      [| 0 <= Z.of_N va + z |]%Z **
+      [| ptr_vaddr (p ,, o) = Some (Z.to_N (Z.of_N va + z)) |].
+
+    Axiom offset_inv_pinned_ptr_pure : forall σ o z va p,
+      eval_offset σ o = Some z ->
+      ptr_vaddr (p ,, o) = Some va ->
+      valid_ptr (p ,, o) |--
+      [| 0 <= Z.of_N va - z |]%Z **
+      [| ptr_vaddr p = Some (Z.to_N (Z.of_N va - z)) |].
+
+    Axiom provides_storage_same_address : forall `{genv} storage_ptr obj_ptr ty,
+      Observe [| same_address storage_ptr obj_ptr |] (provides_storage storage_ptr obj_ptr ty).
+
+    Axiom provides_storage_valid_storage_ptr : forall storage_ptr obj_ptr aty,
+      Observe (valid_ptr storage_ptr) (provides_storage storage_ptr obj_ptr aty).
+    Axiom provides_storage_valid_obj_ptr : forall storage_ptr obj_ptr aty,
+      Observe (valid_ptr obj_ptr) (provides_storage storage_ptr obj_ptr aty).
+
+    #[global] Existing Instances provides_storage_same_address
+      provides_storage_valid_storage_ptr provides_storage_valid_obj_ptr.
+
+  End with_cpp_logic.
+
+    (**
+    [exposed_aid aid] states that the storage instance identified by [aid] is
+    "exposed" [1]. This enables int2ptr casts to produce pointers into this
+    storage instance.
+
+    [1] We use "exposed" in the sense defined by the N2577 draft C standard
+    (http://www.open-std.org/jtc1/sc22/wg14/www/docs/n2577.pdf).
+    See https://dl.acm.org/doi/10.1145/3290380 for an introduction.
+    *)
+    Parameter exposed_aid : forall `{!cpp_logic thread_info Σ}, alloc_id -> mpred.
+
+  Section with_cpp_logic.
+  Context `{cpp_logic}.
+
+    Axiom exposed_aid_persistent : forall aid, Persistent (exposed_aid aid).
+    Axiom exposed_aid_affine : forall aid, Affine (exposed_aid aid).
+    Axiom exposed_aid_timeless : forall aid, Timeless (exposed_aid aid).
+
+    Axiom exposed_aid_null_alloc_id : |-- exposed_aid null_alloc_id.
+
+    #[global] Existing Instances
+      exposed_aid_persistent exposed_aid_affine exposed_aid_timeless.
+
+  End with_cpp_logic.
+
+    (**
+      [type_ptr {resolve := resolve} ty p] asserts that [p] points to
+      a (possibly dead) object of type [ty] (in environment
+      [resolve]), as defined by https://eel.is/c++draft/basic.compound#3.1.
+
+      This implies:
+      - the pointer is strictly valid [type_ptr_strict_valid], and
+        "p + 1" is also valid (while possibly past-the-end) [type_ptr_valid_plus_one].
+      - the pointer is not (an offset of) null pointers [type_ptr_off_nonnull, type_ptr_nonnull]
+      - the pointer is properly aligned [type_ptr_aligned_pure]
+
+      [type_ptr] is persistent and survives deallocation of the pointed-to
+      object, like [_valid_ptr].
+
+      TODO: before a complete object is fully initialized,
+      what [type_ptr] facts are available? For now, we only use [type_ptr]
+      for fully initialized objects.
+      Consider http://eel.is/c++draft/basic.memobj#basic.life, especially
+      from http://eel.is/c++draft/basic.memobj#basic.life-1 to
+      http://eel.is/c++draft/basic.memobj#basic.life-4.
+     *)
+    Parameter type_ptr : forall `{!cpp_logic thread_info Σ} {resolve : genv} (c: Rtype), ptr -> mpred.
+
+  Section with_cpp_logic.
+  Context `{cpp_logic}.
+
+    Axiom type_ptr_persistent : forall {σ} p ty,
+      Persistent (type_ptr ty p).
+    Axiom type_ptr_affine : forall {σ} p ty,
+      Affine (type_ptr ty p).
+    Axiom type_ptr_timeless : forall {σ} p ty,
+      Timeless (type_ptr ty p).
+    #[global] Existing Instances type_ptr_persistent type_ptr_affine type_ptr_timeless.
+
+    Axiom type_ptr_erase : forall {σ} ty p,
+        type_ptr ty p -|- type_ptr (erase_qualifiers ty) p.
+
+    Axiom type_ptr_aligned_pure : forall {σ} ty p,
+      type_ptr ty p |-- [| aligned_ptr_ty ty p |].
+
+    Axiom type_ptr_off_nonnull : forall {σ} ty p o,
+      type_ptr ty (p ,, o) |-- [| p <> nullptr |].
+
+    Axiom tptsto_type_ptr : forall {σ : genv} ty q p v,
+      Observe (type_ptr ty p) (tptsto ty q p v).
+    #[global] Existing Instance tptsto_type_ptr.
+
+    (* All objects in the C++ abstract machine have a size
+
+       NOTE to support un-sized objects, we can simply say that the [sizeof] operator
+            in C++ is only a conservative approximation of the true size of an object.
+     *)
+    Axiom type_ptr_size : forall σ ty p,
+        type_ptr ty p |-- [| is_Some (size_of σ ty) |].
+
+    (**
+    Recall that [type_ptr] and [strict_valid_ptr] don't include
+    past-the-end pointers... *)
+    Axiom type_ptr_strict_valid : forall resolve ty p,
+      type_ptr ty p |-- strict_valid_ptr p.
+    (** Hence they can be incremented into (possibly past-the-end) valid pointers. *)
+    Axiom type_ptr_valid_plus_one : forall `{genv} ty p,
+      type_ptr ty p |-- valid_ptr (p ,, o_sub ty 1).
+
+    (* When [p] is a [ptr] to a C++ object of type [ty], [p] is /also/ a pointer
+       to the "object representation" of [ty] - which consists of "the sequence
+       of [sizeof(ty)] unsigned char objects taken up by the object of
+       type [ty]" [1].
+
+       Detailed Justification:
+       a) From the comment above the axiomatization of [type_ptr]:
+          | [type_ptr ty p] asserts that [p] points to a (possibly dead) object of type [ty].
+       b) In [basic.types.general#4] [1] the C++ Standard states that:
+          | The object representation of an object of type T is the sequence of N unsigned
+          | char objects taken up by the object of type T, where N equals sizeof(T).
+       d) (NOTE: the C++ Standard lacks language regarding this point) the "object representation"
+          for an object pointed to by [ptr] [p] is /also/ accessible via [p].
+       e) (a)+(b)+(d) implies that a (potentially dead) object representation for type [ty]
+          exists at [ptr] [p]
+       f) (a)+(c)+(e) implies that [type_ptr Tbyte (p .[ Tbyte ! i ])] holds (regardless of whether
+          not the object/"object representation" is alive)
+
+       NOTE: There is no need to deal with past-the-end pointers explicitly since
+       [type_ptr] explicitly excludes them; validity of past-the-end pointers
+       can be established using [type_ptr_valid_plus_one].
+
+       [1] <https://eel.is/c++draft/basic.types.general#4>
+     *)
+    Section type_ptr_object_representation.
+      (* This section is intended to axiomatize a /sufficient/ and /sound/
+         set of transport rules for [type_ptr] facts which can be used to
+         satisfy the preconditions required when using [ptr_congP] to
+         transport other resources.
+       *)
+
+      (* The following [Axiom] reflects a trivially faithful encoding of
+         the quote from the C++ standard above [Section type_ptr_object_representation].
+
+         NOTE: To practically use this [Axiom], [type_ptr] must be [Persistent];
+         a reasonable alternative axiomatization which sidestepts this issue
+         could produce /all/ of the [type_ptr] facts for the "object representation"
+         at once:
+         | ... ->
+         |     type_ptr ty p
+         | |-- [∗list] i ∈ seqN 0 (sizeof ty), type_ptr Tbyte (p .[ Tbyte ! i ])
+       *)
+      Section conservative.
+        Axiom type_ptr_obj_repr_byte :
+          forall (σ : genv) (ty : Rtype) (p : ptr) (i sz : N),
+            size_of σ ty = Some sz -> (* 1) [ty] has some byte-size [sz] *)
+            (i < sz)%N ->             (* 2) by (1), [sz] is nonzero and [i] is a
+                                            byte-offset into the object rooted at [p ,, o]
+
+                                         NOTE: [forall ty, size_of (Tarray ty 0) = Some 0],
+                                         but zero-length arrays are not permitted by the Standard
+                                         (cf. <https://eel.is/c++draft/dcl.array#def:array,bound>).
+                                         NOTE: if support for flexible array members is ever added,
+                                         it will need to be carefully coordinated with these sorts
+                                         of transport lemmas.
+                                       *)
+            (* 4) The existence of the "object representation" of an object of type [ty] -
+               |  in conjunction with the premises - justifies "lowering" any
+               |  [type_ptr ty p] fact to a collection of [type_ptr Tbyte (p ,, .[Tbyte ! i])]
+               |  facts - where [i] is a byte-offset within the [ty] ([0 <= i < sizeof(ty)]).
+               v *)
+            type_ptr ty p |-- type_ptr Tbyte (p ,, .[ Tbyte ! i ]).
+      End conservative.
+
+      (* NOTE: This might be reasonable to axiomatize directly; cf. the [NOTE] above
+         [Section conservative].
+       *)
+      Section all_at_once.
+        Lemma type_ptr_obj_repr :
+          forall (σ : genv) (ty : Rtype) (p : ptr) (sz : N),
+            size_of σ ty = Some sz ->
+            type_ptr ty p |-- [∗list] i ∈ seqN 0 sz, type_ptr Tbyte (p .[ Tbyte ! Z.of_N i ]).
+        Proof.
+          intros * Hsz; iIntros "#tptr".
+          iApply big_sepL_intro; iIntros "!>" (k n) "%Hn'".
+          assert (lookup (K:=N) (N.of_nat k) (seqN 0%N sz) = Some n)
+            as Hn
+            by (unfold lookupN, list_lookupN; rewrite Nat2N.id //);
+            clear Hn'.
+          apply lookupN_seqN in Hn as [? ?].
+          iDestruct (type_ptr_obj_repr_byte σ ty p n sz Hsz ltac:(lia) with "tptr") as "$".
+        Qed.
+      End all_at_once.
+    End type_ptr_object_representation.
+
+    (* [offset_congP] hoists [offset_cong] to [mpred] *)
+    Definition offset_congP (σ : genv) (o1 o2 : offset) : mpred :=
+      [| offset_cong σ o1 o2 |].
+
+    (* [ptr_congP σ p1 p2] is an [mpred] which quotients [ptr_cong σ p1 p2]
+       by requiring that [type_ptr Tbyte] holds for both [p1] /and/ [p2]. This property
+       is intended to be sound and sufficient for transporting certain physical
+       resources between [p1] and [p2] - and we hypothesize that it is also
+       necessary.
+     *)
+    Definition ptr_congP (σ : genv) (p1 p2 : ptr) : mpred :=
+      [| ptr_cong σ p1 p2 |] ** type_ptr Tbyte p1 ** type_ptr Tbyte p2.
+
+    (* All [tptsto Tbyte] facts can be transported over [ptr_congP] [ptr]s.
+
+       High level meaning:
+       In the C++ object model, a single byte of storage can be accessed through different pointers,
+       e.g. consider [struct C { int x; int y; } c;]. The first byte of the struct can be read through
+       [static_cast<byte*>(&c)] (with pointer representation [c]) as well as [static_cast<byte*>(&c.x)]
+       (with pointer representation [c ,, _field "::C" "x"]). To put an ownership discipline on this
+       single byte, we build an equivalence relation on pointers that allows us to transport ownership
+       of the byte between these different pointers. For example, half of the ownership could live at [c]
+       and the other half of the ownership can live at [c ,, _field "::C" "x"].
+
+       The standard justifies this as follows:
+       1) (cf. [tptsto] comment) [tptsto ty q p v] ensures that [p] points to a memory
+          location with C++ type [ty] and which has some value [v].
+       2) (cf. [Section type_ptr_object_representation]) [type_ptr Tbyte] holds for all of the
+          bytes (i.e. the "object reprsentation") constituting well-typed C++ objects.
+       3) NOTE (JH): the following isn't quite true yet, but we'll want this when we flesh
+          out [rawR]/[RAW_BYTES]:
+          a) all values [v] can be converted into (potentially many) [raw_byte]s -
+             which capture its "object representation"
+          b) all [tptsto ty] facts can be shattered into (potentially many)
+             [tptsto Tbyte _ _ (Vraw _)] facts corresponding to its "object representation"
+       4) [tptsto Tbyte _ _ (Vraw _)] can be transported over [ptr_congP] [ptr]s:
+          a) [tptso Tbyte _ _ (Vraw _)] facts deal with the "object representation" directly
+             and thus permit erasing the structure of pointers in favor of reasoning about
+             relative byte offsets from a shared [ptr]-prefix.
+          b) the [ptr]s are [ptr_congP] so we know that:
+             i) they share a common base pointer [p_base]
+             ii) the byte-offset values of the C++ offsets which reconstitute the src/dst from
+                 [p_base] are equal
+             iii) NOTE: (cf. [valid_ptr_nonnull_nonzero]/[type_ptr_valid_ptr]/[type_ptr_nonnull] below)
+                  [p_base] has some [vaddr], but we don't currently rely on this fact.
+     *)
+    (* TODO: improve our axiomatic support for raw values - including "shattering"
+       non-raw values into their constituent raw pieces - to enable deriving
+       [tptsto_ptr_congP_transport] from [tptsto_raw_ptr_congP_transport].
+     *)
+    Axiom tptsto_ptr_congP_transport : forall {σ} q p1 p2 v,
+      ptr_congP σ p1 p2 |-- tptsto (σ:=σ) Tbyte q p1 v -* tptsto (σ:=σ) Tbyte q p2 v.
+
+    (**
+     ** Deducing pointer equalities
+     The following axioms, together with [same_address_o_sub_eq], enable going
+     from [same_address] (produced by C++ pointer equality) to actual pointer
+     equalities.
+     *)
+
+    (** Pointer equality with [nullptr] is easy, as long as your pointer is valid.
+     Validity is necessary: the C++ expression [(char * )p - (uintptr_t) p]
+     produces an invalid pointer with address 0, which is not [nullptr] because
+     it preserves the provenance of [p]. *)
+    Axiom same_address_eq_null : forall `{genv} p tv,
+      _valid_ptr tv p |--
+      [| same_address p nullptr <-> p = nullptr |].
+
+    (**
+    [same_address_eq_type_ptr] concludes that two pointers [p1] and [p2] are
+    equal if they have the same address, point to live objects [o1] and [o2],
+    and have the same (non-uchar) type [ty] with nonzero size.
+
+    Justifying this from the standard is tricky; here's a proof sketch.
+    - Because [ty] has "nonzero size" (https://eel.is/c++draft/intro.object#8),
+      and we don't support bitfields, we apply the standard:
+
+      > Unless it is a bit-field, an object with nonzero size shall occupy one
+        or more bytes of storage, including every byte that is occupied in full
+        or in part by any of its subobjects.
+
+    - Because [o1] and [o2] are live, these objects share storage, hence they
+      must coincide or one must be nested inside the other
+      (https://eel.is/c++draft/intro.object#4); if they coincide, our proof
+      is done.
+    - Because [ty] is not [unsigned char], neither pointer can provide storage
+      for the other (https://eel.is/c++draft/intro.object#3); so one must be a
+      subobject of the other.
+    - Since [o1] and [o2] have type [ty], and type [ty] has "nonzero size",
+      neither of [o1] and [o2] can be a subobject of the other;
+      we conjecture is provable from the C++ type system.
+
+    NOTE: we check "nonzero size"
+    (https://eel.is/c++draft/basic.memobj#intro.object-8) using [size_of],
+    which might incorporate implementation-specific compiler decisions.
+    TODO: handle [std::byte] like [unsigned char].
+    *)
+    Axiom same_address_eq_type_ptr : forall resolve ty p1 p2 n,
+      same_address p1 p2 ->
+      size_of resolve ty = Some n ->
+      (* if [ty = Tuchar], one of these pointer could provide storage for the other. *)
+      ty <> Tuchar ->
+      (n > 0)%N ->
+      type_ptr ty p1 ∧ type_ptr ty p2 ∧ live_ptr p1 ∧ live_ptr p2 ⊢
+        |={↑pred_ns}=> [| p1 = p2 |].
+
+  End with_cpp_logic.
+
+    (** Padding
+        [struct_padding] and [union_padding] represent the object state of an aggregate.
+        Ownership of this token implies that the object is a alive. They only given when
+        an object is fully constructed, and are taken back at the end of the lifetime.
+        This is related to the "construction state" in Tahina's work, i.e.
+        <https://inria.hal.science/file/index/docid/674663/filename/cpp-construction.pdf>
+     *)
+    Axiom struct_padding : forall `{!cpp_logic thread_info Σ} {σ:genv},
+      ptr -> globname -> cQp.t -> mpred.
+
+  Section with_cpp_logic.
+  Context `{cpp_logic}.
+
+    #[global] Declare Instance struct_padding_timeless {σ:genv} : Timeless3 (struct_padding).
+    #[global] Declare Instance struct_padding_fractional : forall {σ : genv} p cls, CFractional (struct_padding p cls).
+    #[global] Declare Instance struct_padding_frac_valid : forall {σ : genv} p cls, CFracValid0 (struct_padding p cls).
+
+    #[global] Declare Instance struct_padding_type_ptr_observe : forall {σ : genv} p cls q,
+        Observe (type_ptr (Tnamed cls) p) (struct_padding p cls q).
+
+  End with_cpp_logic.
+
+    (** [union_padding cls q active_member] is [q] ownership of
+     the union padding for union [cls] for the active member
+     [active_member]. When there is no active member the [active_member]
+     is [None], otherwise it is [Some idx] where [idx] is the numeric
+     index of member field.
+     *)
+    Axiom union_padding : forall `{!cpp_logic thread_info Σ} {σ:genv},
+      ptr -> globname -> cQp.t -> option nat -> mpred.
+
+  Section with_cpp_logic.
+  Context `{cpp_logic}.
+
+    #[global] Declare Instance union_padding_timeless {σ:genv} :  Timeless4 (union_padding).
+    #[global] Declare Instance union_padding_fractional : forall {σ : genv} p cls, CFractional1 (union_padding p cls).
+    #[global] Declare Instance union_padding_frac_valid : forall {σ : genv} p cls, CFracValid1 (union_padding p cls).
+
+    #[global] Declare Instance union_padding_type_ptr_observe : forall {σ : genv} p cls q active,
+        Observe (type_ptr (Tnamed cls) p) (union_padding p cls q active).
+    #[global] Declare Instance union_padding_agree : forall {σ : genv} p cls q q' i i',
+        Observe2 [| i = i' |] (union_padding p cls q i) (union_padding p cls q' i').
+
+  End with_cpp_logic.
+
+  End with_cpp.
+
+  (* strict validity (not past-the-end) *)
+  Notation strict_valid_ptr := (_valid_ptr Strict).
+  (* validity (past-the-end allowed) *)
+  Notation valid_ptr := (_valid_ptr Relaxed).
+End CPP_LOGIC.
+
+(* Pointer axioms. XXX Not modeled for now. *)
+Module Type VALID_PTR_AXIOMS
+  (Import P : PTRS_INTF)
+  (Import INTF : VALUES_INTF_FUNCTOR P)
+  (Import CC : CPP_LOGIC_CLASS)
+  (Import CPP : CPP_LOGIC P INTF CC).
+
+  Implicit Types (p : ptr).
+
+  Section with_cpp.
+    Context `{cpp_logic} {σ : genv}.
+
+    Axiom invalid_ptr_invalid : forall vt,
+      _valid_ptr vt invalid_ptr |-- False.
+
+    (** Justified by [https://eel.is/c++draft/expr.add#4.1]. *)
+    Axiom _valid_ptr_nullptr_sub_false : forall vt ty (i : Z) (_ : i <> 0),
+      _valid_ptr vt (nullptr ,, o_sub ty i) |-- False.
+    (*
+    TODO Controversial; if [f] is the first field, [nullptr->f] or casts relying on
+    https://eel.is/c++draft/basic.compound#4 might invalidate this.
+    To make this valid, we could ensure our axiomatic semantics produces
+    [nullptr] instead of [nullptr ., o_field]. *)
+    (* Axiom _valid_ptr_nullptr_field_false : forall vt f,
+      _valid_ptr vt (nullptr ,, o_field σ f) |-- False. *)
+
+    (** These axioms are named after the predicate in the conclusion. *)
+
+    (**
+    TODO: The intended proof of [strict_valid_ptr_sub] assumes that, if [p']
+    normalizes to [p ., [ ty ! i ]], then [valid_ptr p'] is defined to imply
+    validity of all pointers from [p] to [p'].
+
+    Note that `arrR` exposes stronger reasoning principles, but this might still be useful.
+    *)
+    Axiom strict_valid_ptr_sub : ∀ (i j k : Z) p ty vt1 vt2,
+      (i <= j < k)%Z ->
+      _valid_ptr vt1 (p ,, o_sub ty i) |--
+      _valid_ptr vt2 (p ,, o_sub ty k) -* strict_valid_ptr (p ,, o_sub ty j).
+
+    (** XXX: this axiom is convoluted but
+    TODO: The intended proof of [strict_valid_ptr_field_sub] (and friends) is that
+    (1) if [p'] normalizes to [p'' ., [ ty ! i ]], then [valid_ptr p'] implies
+    [valid_ptr p''].
+    (2) [p ,, o_field σ f ,, o_sub σ ty i] will normalize to [p ,, o_field
+    σ f ,, o_sub σ ty i], without cancellation.
+    *)
+    Axiom strict_valid_ptr_field_sub : ∀ (p : ptr) ty (i : Z) f vt,
+      (0 < i)%Z ->
+      _valid_ptr vt (p ,, o_field f ,, o_sub ty i) |-- strict_valid_ptr (p ,, o_field f).
+
+    (* TODO: can we deduce that [p] is strictly valid? *)
+    Axiom _valid_ptr_field : ∀ p f vt,
+      _valid_ptr vt (p ,, o_field f) |-- _valid_ptr vt p.
+    (* TODO: Pointers to fields can't be past-the-end, right?
+    Except 0-size arrays. *)
+    (* Axiom strict_valid_ptr_field : ∀ p f,
+      valid_ptr (p ,, o_field σ f) |--
+      strict_valid_ptr (p ,, o_field σ f). *)
+    (* TODO: if we add [strict_valid_ptr_field], we can derive
+    [_valid_ptr_field] from just [strict_valid_ptr_field] *)
+    (* Axiom strict_valid_ptr_field : ∀ p f,
+      strict_valid_ptr (p ,, o_field σ f) |-- strict_valid_ptr p. *)
+
+    (* We're ignoring virtual inheritance here, since we have no plans to
+    support it for now, but this might hold there too. *)
+    Axiom o_base_directly_derives : forall p base derived,
+      strict_valid_ptr (p ,, o_base derived base) |--
+      [| directly_derives σ derived base |].
+
+    Axiom o_derived_directly_derives : forall p base derived,
+      strict_valid_ptr (p ,, o_derived base derived) |--
+      [| directly_derives σ derived base |].
+
+    (* TODO: maybe add a validity of offsets to allow stating this more generally. *)
+    Axiom valid_o_sub_size : forall p ty i vt,
+      _valid_ptr vt (p ,, o_sub ty i) |-- [| is_Some (size_of σ ty) |].
+
+    Axiom type_ptr_o_base : forall derived base p,
+      class_derives derived [base] ->
+      type_ptr (Tnamed derived) p ⊢ type_ptr (Tnamed base) (p ,, _base derived base).
+
+    (*
+    Axiom type_ptr_o_field_type_ptr : forall p fld cls st,
+      glob_def σ cls = Some (Gstruct st) ->
+      fld ∈ s_fields st →
+         type_ptr (Tnamed cls) p
+      ⊢ type_ptr fld.(mem_type) (p ., Field cls fld.(mem_name)). (* TODO field names *)
+      *)
+
+    Axiom type_ptr_o_sub : forall p (m n : N) ty,
+      (m < n)%N ->
+      type_ptr (Tarray ty n) p ⊢ type_ptr ty (p ,, _sub ty m).
+  End with_cpp.
+End VALID_PTR_AXIOMS.
+
+Declare Module L : CPP_LOGIC PTRS_INTF_AXIOM VALUES_INTF_AXIOM LC.
+Export L.
+
+Declare Module Export VALID_PTR : VALID_PTR_AXIOMS PTRS_INTF_AXIOM VALUES_INTF_AXIOM LC L.
+
+Section valid_ptr_code.
+  Context `{cpp_logic} {σ : genv} (tu : translation_unit).
+
+  Lemma code_at_valid   : forall f p,   code_at tu f p |-- valid_ptr p.
+  Proof. intros. rewrite code_at_strict_valid; apply strict_valid_valid. Qed.
+  Lemma method_at_valid : forall f p, method_at tu f p |-- valid_ptr p.
+  Proof. intros. rewrite method_at_strict_valid; apply strict_valid_valid. Qed.
+  Lemma ctor_at_valid   : forall f p,   ctor_at tu f p |-- valid_ptr p.
+  Proof. intros. rewrite ctor_at_strict_valid; apply strict_valid_valid. Qed.
+  Lemma dtor_at_valid   : forall f p,   dtor_at tu f p |-- valid_ptr p.
+  Proof. intros. rewrite dtor_at_strict_valid; apply strict_valid_valid. Qed.
+End valid_ptr_code.
+
+mlock Definition exposed_ptr `{cpp_logic} p : mpred :=
+  valid_ptr p ** ∃ aid, [| ptr_alloc_id p = Some aid |] ** exposed_aid aid.
+#[global] Arguments exposed_ptr {_ _ _} p : assert.
+
+(** Physical representation of pointers. *)
+(** [pinned_ptr va p] states that the abstract pointer [p] is tied to a
+  virtual address [va].
+  [pinned_ptr] will only hold on pointers that are associated to addresses,
+  but other pointers exist. *)
+(* mlock Definition pinned_ptr `{cpp_logic} (va : vaddr) (p : ptr) : mpred :=
+  [| ptr_vaddr p = Some va |] ** exposed_ptr p.
+#[global] Arguments pinned_ptr {_ _ _} va p : assert.
+
+Notation pinned_ptr_Z va p :=
+  ([| 0 <= va |]%Z ** pinned_ptr (Z.to_N va) p).
+
+Section pinned_ptr_def.
+  Context `{cpp_logic}.
+
+  #[global] Instance exposed_ptr_persistent p : Persistent (exposed_ptr p).
+  Proof. rewrite exposed_ptr.unlock. apply _. Qed.
+  #[global] Instance exposed_ptr_affine p : Affine (exposed_ptr p).
+  Proof. rewrite exposed_ptr.unlock. apply _. Qed.
+  #[global] Instance exposed_ptr_timeless p : Timeless (exposed_ptr p).
+  Proof. rewrite exposed_ptr.unlock. apply _. Qed.
+  #[global] Instance exposed_ptr_valid p :
+    Observe (valid_ptr p) (exposed_ptr p).
+  Proof. rewrite exposed_ptr.unlock. apply _. Qed.
+
+  Lemma exposed_ptr_nullptr : |-- exposed_ptr nullptr.
+  Proof.
+    rewrite exposed_ptr.unlock ptr_alloc_id_nullptr.
+    iDestruct valid_ptr_nullptr as "$". iExists _.
+    by iDestruct exposed_aid_null_alloc_id as "$".
+  Qed.
+
+  Lemma offset2_exposed_ptr p o1 o2 :
+    valid_ptr (p ,, o2) |-- exposed_ptr (p ,, o1) -* exposed_ptr (p ,, o2).
+  Proof.
+    rewrite exposed_ptr.unlock.
+    iIntros "#V2 #[V1 E]"; iFrame "V2".
+    iDestruct (valid_ptr_alloc_id with "V1") as %?.
+    iDestruct (valid_ptr_alloc_id with "V2") as %?.
+    by rewrite ptr_alloc_id_offset // ptr_alloc_id_offset.
+  Qed.
+
+  Lemma offset_exposed_ptr p o :
+    valid_ptr (p ,, o) |-- exposed_ptr p -* exposed_ptr (p ,, o).
+  Proof. rewrite -{2}(offset_ptr_id p). apply offset2_exposed_ptr. Qed.
+
+  Lemma offset_inv_exposed_ptr p o :
+    valid_ptr p |-- exposed_ptr (p ,, o) -* exposed_ptr p.
+  Proof. rewrite -{1 3}(offset_ptr_id p). apply offset2_exposed_ptr. Qed.
+
+  Lemma offset_exposed_ptr_all p o :
+    valid_ptr p ∗ valid_ptr (p ,, o) ⊢ exposed_ptr p ∗-∗ exposed_ptr (p ,, o).
+  Proof.
+    iIntros "#[V V']"; iSplit.
+    by iApply offset_exposed_ptr.
+    by iApply offset_inv_exposed_ptr.
+  Qed.
+
+  #[global] Instance pinned_ptr_persistent va p : Persistent (pinned_ptr va p).
+  Proof. rewrite pinned_ptr.unlock. apply _. Qed.
+  #[global] Instance pinned_ptr_affine va p : Affine (pinned_ptr va p).
+  Proof. rewrite pinned_ptr.unlock. apply _. Qed.
+  #[global] Instance pinned_ptr_timeless va p : Timeless (pinned_ptr va p).
+  Proof. rewrite pinned_ptr.unlock. apply _. Qed.
+
+  Lemma pinned_ptr_intro p va :
+    ptr_vaddr p = Some va -> exposed_ptr p |-- pinned_ptr va p.
+  Proof. rewrite pinned_ptr.unlock. by iIntros (?) "$". Qed.
+
+  #[global] Instance pinned_ptr_ptr_vaddr va p :
+    Observe [| ptr_vaddr p = Some va |] (pinned_ptr va p).
+  Proof. rewrite pinned_ptr.unlock. apply _. Qed.
+
+  Lemma pinned_ptr_change_va_eq (p : ptr) (va va' : vaddr)
+    (Heq : ptr_vaddr p = Some va) :
+    pinned_ptr va' p |--  [| va' = va |] ** pinned_ptr va p.
+  Proof.
+    iIntros "#P".
+    iDestruct (observe_elim_pure (ptr_vaddr p = Some va') with "P") as %?.
+    simplify_eq. auto.
+  Qed.
+
+  Lemma pinned_ptr_change_va p va va'
+    (Heq : ptr_vaddr p = Some va) :
+    pinned_ptr va' p |-- pinned_ptr va p.
+  Proof. rewrite pinned_ptr_change_va_eq //. by iIntros "[_ $]". Qed.
+
+  #[global] Instance pinned_ptr_agree va1 va2 p :
+    Observe2 [| va1 = va2 |] (pinned_ptr va1 p) (pinned_ptr va2 p).
+  Proof.
+    iIntros "#P1 #P2 !>".
+    iDestruct (observe_elim_pure (_ = _) with "P1") as %?.
+    iDestruct (observe_elim_pure (_ = _) with "P2") as %?; simplify_eq.
+    by [].
+  Qed.
+
+  #[global] Instance pinned_ptr_valid va p :
+    Observe (valid_ptr p) (pinned_ptr va p).
+  Proof. rewrite pinned_ptr.unlock. apply _. Qed.
+
+  (** Just a corollary of [provides_storage_same_address] in the style of
+  [provides_storage_pinned_ptr]. *)
+  Lemma provides_storage_pinned_ptr_pure {storage_ptr obj_ptr aty va} :
+    ptr_vaddr storage_ptr = Some va ->
+    provides_storage storage_ptr obj_ptr aty |-- [| ptr_vaddr obj_ptr = Some va |].
+  Proof. rewrite provides_storage_same_address. by iIntros (HP <-). Qed.
+End pinned_ptr_def.
+
+Section with_cpp.
+  Context `{cpp_logic} {σ : genv}.
+
+  Lemma same_address_bool_null p tv :
+    _valid_ptr tv p |--
+    [| same_address_bool p nullptr = bool_decide (p = nullptr) |].
+  Proof. rewrite same_address_eq_null; iIntros "!%". apply bool_decide_ext. Qed.
+
+  Lemma valid_ptr_zero_null p :
+    ptr_vaddr p = Some 0%N ->
+    valid_ptr p |-- [| p = nullptr |].
+  Proof.
+    rewrite same_address_eq_null.
+    iIntros (Haddr [Hsuff _]) "!%". apply: Hsuff.
+    rewrite same_address_iff ptr_vaddr_nullptr; naive_solver.
+  Qed.
+
+  Lemma valid_ptr_nonnull_nonzero p :
+    p <> nullptr ->
+    valid_ptr p |-- [| ptr_vaddr p <> Some 0%N |].
+  Proof.
+    destruct (decide (ptr_vaddr p = Some 0%N)); last naive_solver.
+    rewrite valid_ptr_zero_null; naive_solver.
+  Qed.
+
+  Lemma type_ptr_nonnull ty p :
+    type_ptr ty p |-- [| p <> nullptr |].
+  Proof. rewrite -{1}(offset_ptr_id p). apply type_ptr_off_nonnull. Qed.
+
+  #[global] Instance type_ptr_observe_nonnull ty p :
+    Observe [| p <> nullptr |] (type_ptr ty p).
+  Proof. rewrite type_ptr_nonnull. refine _. Qed.
+
+  #[global] Instance provides_storage_preserves_nullptr {storage_ptr obj_ptr aty} :
+    Observe [| storage_ptr = nullptr <-> obj_ptr = nullptr |] (provides_storage storage_ptr obj_ptr aty).
+  Proof.
+    apply observe_intro_only_provable; iIntros "PS".
+    iDestruct (provides_storage_same_address with "PS") as %Hsm.
+    iDestruct (provides_storage_valid_obj_ptr with "PS") as "#VO".
+    iDestruct (provides_storage_valid_storage_ptr with "PS") as "#VS {PS}".
+    iDestruct (same_address_eq_null with "VO") as %[HeqO _].
+    iDestruct (same_address_eq_null with "VS") as %[HeqS _].
+    iIntros "!%"; split; intros ->.
+    - apply HeqO, symmetry, Hsm.
+    - apply HeqS, Hsm.
+  Qed.
+
+  #[global] Instance provides_storage_preserves_nonnull {storage_ptr obj_ptr aty} :
+    Observe [| storage_ptr <> nullptr <-> obj_ptr <> nullptr |] (provides_storage storage_ptr obj_ptr aty).
+  Proof.
+    apply observe_intro_only_provable. iIntros "PS".
+    by iDestruct (provides_storage_preserves_nullptr with "PS") as "#-> {PS}".
+  Qed.
+
+  #[global] Instance pinned_ptr_unique va va' p :
+    Observe2 [| va = va' |] (pinned_ptr va p) (pinned_ptr va' p).
+  Proof.
+    rewrite pinned_ptr.unlock.
+    iIntros "[%H1 _] [%H2 _] !> !%". congruence.
+  Qed.
+
+  Lemma offset_2_pinned_ptr_pure o1 o2 z1 z2 va p :
+    eval_offset σ o1 = Some z1 ->
+    eval_offset σ o2 = Some z2 ->
+    ptr_vaddr (p ,, o1) = Some va ->
+    valid_ptr p |-- valid_ptr (p ,, o1) -* valid_ptr (p ,, o2) -*
+    [| 0 <= Z.of_N va - z1 + z2 |]%Z **
+    [| ptr_vaddr (p ,, o2) = Some (Z.to_N (Z.of_N va - z1 + z2)) |].
+  Proof.
+    iIntros (He1 He2 Hpin1) "V V1 V2".
+    iDestruct (offset_inv_pinned_ptr_pure with "V1") as %[Hle1 Hp]; [done..|].
+    iDestruct (offset_pinned_ptr_pure with "V2") as %[Hle2 Hgoal]; [done..|].
+    iIntros "!%". by rewrite Z2N.id in Hgoal, Hle2.
+  Qed.
+
+  Lemma pinned_ptr_null : |-- pinned_ptr 0 nullptr.
+  Proof.
+    rewrite pinned_ptr.unlock.
+    iFrame (ptr_vaddr_nullptr).
+    iApply exposed_ptr_nullptr.
+  Qed.
+
+  #[global] Instance pinned_ptr_zero_is_null (p : ptr) :
+    Observe [| p = nullptr |] (pinned_ptr 0 p).
+  Proof.
+    rewrite pinned_ptr.unlock.
+    iIntros "[%Heq #E]".
+    rewrite -valid_ptr_zero_null //.
+    by iApply (exposed_ptr_valid with "E").
+  Qed.
+
+  #[global] Instance pinned_ptr_null_is_zero addr :
+    Observe [| addr = 0 |]%N (pinned_ptr addr nullptr).
+  Proof.
+    rewrite pinned_ptr.unlock ptr_vaddr_nullptr.
+    apply: (observe_derive_only_provable (Some 0%N = Some addr)); naive_solver.
+  Qed.
+
+  Lemma pinned_ptr_same_address pp1 pp2 v :
+    same_address pp1 pp2 ->
+    exposed_ptr pp2 |-- pinned_ptr v pp1 -* pinned_ptr v pp2.
+  Proof.
+    rewrite pinned_ptr.unlock.
+    by iIntros ((? & -> & ->)%same_address_iff) "$ [%Hp _] !%".
+  Qed.
+
+  Lemma offset_pinned_ptr_Z o z va p :
+    eval_offset _ o = Some z ->
+    valid_ptr (p ,, o) |--
+    pinned_ptr va p -*
+    pinned_ptr_Z (Z.of_N va + z) (p ,, o).
+  Proof.
+    rewrite pinned_ptr.unlock.
+    iIntros (He) "#V' #(%P & E)".
+    iDestruct (offset_pinned_ptr_pure with "V'") as "[$ $]"; [done..|].
+    by iApply offset_exposed_ptr.
+  Qed.
+
+  Lemma offset_pinned_ptr o z va p :
+    eval_offset _ o = Some z ->
+    valid_ptr (p ,, o) |--
+    pinned_ptr va p -*
+    pinned_ptr (Z.to_N (Z.of_N va + z)) (p ,, o).
+  Proof.
+    iIntros (?) "V P".
+    by iDestruct (offset_pinned_ptr_Z with "V P") as "[_ $]".
+  Qed.
+
+  Lemma offset_inv_pinned_ptr_Z o z va p :
+    eval_offset _ o = Some z ->
+    valid_ptr p |--
+    pinned_ptr va (p ,, o) -*
+    pinned_ptr_Z (Z.of_N va - z) p.
+  Proof.
+    rewrite pinned_ptr.unlock.
+    iIntros (He) "#V #(%P & E)".
+    iDestruct (offset_inv_pinned_ptr_pure with "[]") as "-#[$$]"; [done..| |].
+    { by iApply (observe with "E"). }
+    by iApply offset_inv_exposed_ptr.
+  Qed.
+
+  Lemma offset_2_pinned_ptr_Z o1 o2 z1 z2 va p :
+    eval_offset σ o1 = Some z1 ->
+    eval_offset σ o2 = Some z2 ->
+    valid_ptr p |-- valid_ptr (p ,, o1) -* valid_ptr (p ,, o2) -*
+    pinned_ptr va (p ,, o1) -*
+    pinned_ptr_Z (Z.of_N va - z1 + z2) (p ,, o2).
+  Proof.
+    rewrite pinned_ptr.unlock.
+    iIntros (He1 He2) "V V1 #V2 #(%P & E)".
+    iDestruct (offset_2_pinned_ptr_pure with "V V1 V2") as "[$$]"; [done..|].
+    by iApply offset2_exposed_ptr.
+  Qed.
+
+  Lemma pinned_ptr_aligned_divide va n p :
+    pinned_ptr va p ⊢
+    [| aligned_ptr n p <-> (n | va)%N |].
+  Proof.
+    rewrite pinned_ptr.unlock; iIntros "(%P & _) !%".
+    exact: pinned_ptr_pure_aligned_divide.
+  Qed.
+
+  Lemma pinned_ptr_pure_type_divide_1 va n p ty
+    (Hal : align_of ty = Some n) :
+    type_ptr ty p ⊢ [| ptr_vaddr p = Some va |] -∗ [| (n | va)%N |].
+  Proof.
+    rewrite type_ptr_aligned_pure. iIntros "!%".
+    exact: pinned_ptr_pure_divide_1.
+  Qed.
+
+  Lemma pinned_ptr_type_divide_1 va n p ty
+    (Hal : align_of ty = Some n) :
+    type_ptr ty p ⊢ pinned_ptr va p -∗ [| (n | va)%N |].
+  Proof.
+    rewrite pinned_ptr.unlock.
+    iIntros "#? #(? & _)". by iApply pinned_ptr_pure_type_divide_1.
+  Qed.
+
+  Lemma shift_pinned_ptr_Z_sub ty z va (p1 p2 : ptr) o:
+    p1 ,, o_sub _ ty z = p2 ->
+    size_of σ ty = Some o ->
+        valid_ptr p2 ** pinned_ptr va p1
+    |-- pinned_ptr_Z (Z.of_N va + z * Z.of_N o) p2.
+  Proof.
+    move => <- o_eq.
+    iIntros "[val pin1]".
+    iApply (offset_pinned_ptr_Z with "val") => //.
+    rewrite eval_o_sub o_eq /= Z.mul_comm //.
+  Qed.
+
+  Lemma shift_pinned_ptr_sub ty z va (p1 p2 : ptr) o:
+    p1 ,, o_sub _ ty z = p2 ->
+    size_of σ ty = Some o ->
+        valid_ptr p2 ** pinned_ptr va p1
+    |-- pinned_ptr (Z.to_N (Z.of_N va + z * Z.of_N o)) p2.
+  Proof.
+    iIntros (??) "VP".
+    by iDestruct (shift_pinned_ptr_Z_sub with "VP") as "[_ $]".
+  Qed.
+
+  Lemma _valid_valid p vt : _valid_ptr vt p |-- valid_ptr p.
+  Proof. case: vt => [|//]. exact: strict_valid_valid. Qed.
+
+  Lemma valid_ptr_sub (i j k : Z) p ty vt
+    (Hj : (i <= j <= k)%Z) :
+    _valid_ptr vt (p ,, o_sub σ ty i) |--
+    _valid_ptr vt (p ,, o_sub σ ty k) -* valid_ptr (p ,, o_sub σ ty j).
+  Proof.
+    destruct (decide (j = k)) as [->|Hne].
+    { rewrite -_valid_valid. by iIntros "_ $". }
+    rewrite -strict_valid_valid. apply strict_valid_ptr_sub. lia.
+  Qed.
+
+  Lemma _valid_ptr_field_sub (i : Z) (p : ptr) ty f vt (Hle : (0 <= i)%Z) :
+    _valid_ptr vt (p ,, o_field σ f ,, o_sub σ ty i) |-- _valid_ptr vt (p ,, o_field σ f).
+  Proof.
+    iIntros "V". case: (decide (i = 0)%Z) Hle => [-> _|Hne Hle].
+    - iDestruct (valid_o_sub_size with "V") as %?.
+      by rewrite offset_ptr_sub_0.
+    - rewrite strict_valid_ptr_field_sub; last by lia.
+      case: vt => //. by rewrite strict_valid_valid.
+  Qed.
+
+  Lemma o_base_derived_strict p base derived :
+    strict_valid_ptr (p ,, o_base σ derived base) |--
+    [| p ,, o_base σ derived base ,, o_derived σ base derived = p |].
+  Proof.
+    rewrite o_base_directly_derives. f_equiv => ?. exact: o_base_derived.
+  Qed.
+
+  Lemma o_derived_base_strict p base derived :
+    strict_valid_ptr (p ,, o_derived σ base derived) |--
+    [| p ,, o_derived σ base derived ,, o_base σ derived base = p |].
+  Proof.
+    rewrite o_derived_directly_derives. f_equiv => ?. exact: o_derived_base.
+  Qed.
+
+  Lemma o_derived_base_type p base derived ty :
+    type_ptr ty (p ,, o_derived σ base derived) |--
+    [| p ,, o_derived σ base derived ,, o_base σ derived base = p |].
+  Proof. rewrite type_ptr_strict_valid. apply (o_derived_base_strict p). Qed.
+
+  (** [_inv] because unlike [type_ptr_o_base] and [type_ptr_o_field_type_ptr],
+  this lemma fits the [type_ptr _ (p ,, o) ⊢ type_ptr _ p] schema instead of the
+  converse. *)
+  Lemma type_ptr_o_derived_inv derived base p :
+    class_derives derived [base] ->
+    type_ptr (Tnamed derived) (p ,, _derived base derived) |--
+    type_ptr (Tnamed base) p.
+  Proof.
+    iIntros (Hcd) "T".
+    iDestruct (o_derived_base_type with "T") as %Hp.
+    by rewrite (type_ptr_o_base _ _ _ Hcd) Hp.
+  Qed.
+
+  (** [p] is a valid pointer value in the sense of the standard, or
+  "standard-valid" (https://eel.is/c++draft/basic.compound#3.1), that is both
+  valid (in our sense) and live.
+
+  In particular, [p] is a valid pointer value even when accounting for
+  pointer zapping.
+  *)
+  Definition _valid_live_ptr vt (p : ptr) : mpred :=
+    _valid_ptr vt p ∗ live_ptr p.
+  Definition valid_live_ptr p : mpred := _valid_live_ptr Relaxed p.
+  Definition strict_valid_live_ptr p : mpred := _valid_live_ptr Strict p.
+
+  #[global] Instance tptsto_flip_mono :
+    Proper (flip genv_leq ==> eq ==> eq ==> eq ==> eq ==> flip (⊢))
+      (@tptsto _ _ _).
+  Proof. repeat intro. exact: tptsto_mono. Qed.
+
+  #[global] Instance tptsto_as_cfractional ty : AsCFractional2 (tptsto ty).
+  Proof. solve_as_cfrac. Qed.
+
+  #[global] Instance mdc_path_as_cfractional this mdc :
+    AsCFractional1 (mdc_path this mdc).
+  Proof. solve_as_cfrac. Qed.
+
+  #[global] Instance tptsto_observe_nonnull t q p v :
+    Observe [| p <> nullptr |] (tptsto t q p v).
+  Proof.
+    apply: observe_intro.
+    destruct (decide (p = nullptr)); subst; last by eauto.
+    rewrite {1}tptsto_nonnull. exact: bi.False_elim.
+  Qed.
+
+  Lemma tptsto_disjoint ty c1 c2 q p v1 v2 :
+    tptsto ty (cQp.mk c1 1) p v1 ** tptsto ty (cQp.mk c2 q) p v2 |-- False.
+  Proof.
+    iIntros "[T1 T2]".
+    iDestruct (tptsto_agree with "T1 T2") as %->.
+    iCombine "T1 T2" as "T".
+    by iDestruct (cfrac_valid_2 with "T") as %?%Qp.not_add_le_l.
+  Qed.
+
+  Lemma offset_ptr_congP (p : ptr) o1 o2 :
+    offset_congP σ o1 o2 |--
+    type_ptr Tbyte (p ,, o1) -*
+    type_ptr Tbyte (p ,, o2) -*
+    ptr_congP σ (p ,, o1) (p ,, o2).
+  Proof.
+    iIntros "% T1 T2". rewrite /ptr_congP. iFrame "T1 T2".
+    auto using offset_ptr_cong.
+  Qed.
+
+  (** *** Just wrappers. *)
+  (** We can lift validity entailments through [Observe] (using
+  [Observe_mono]. These are not instances, to avoid causing slowdowns in
+  proof search. *)
+  Lemma observe_strict_valid_valid
+    `(Hobs : !Observe (strict_valid_ptr p) P) : Observe (valid_ptr p) P.
+  Proof. by rewrite -strict_valid_valid. Qed.
+
+  Lemma observe_type_ptr_strict_valid
+    `(Hobs : !Observe (type_ptr ty p) P) : Observe (strict_valid_ptr p) P.
+  Proof. by rewrite -type_ptr_strict_valid. Qed.
+
+  Lemma observe_type_ptr_valid_plus_one
+    `(Hobs : !Observe (type_ptr ty p) P) : Observe (valid_ptr (p ,, o_sub σ ty 1)) P.
+  Proof. by rewrite -type_ptr_valid_plus_one. Qed.
+
+  Lemma type_ptr_valid ty p : type_ptr ty p |-- valid_ptr p.
+  Proof. by rewrite type_ptr_strict_valid strict_valid_valid. Qed.
+
+  Lemma type_ptr__valid ty p vt : type_ptr ty p |-- _valid_ptr vt p.
+  Proof.
+    case: vt.
+    apply type_ptr_strict_valid.
+    apply type_ptr_valid.
+  Qed.
+
+  #[global] Instance type_ptr_size_observe ty p :
+    Observe [| is_Some (size_of σ ty) |] (type_ptr ty p).
+  Proof. rewrite type_ptr_size. apply _. Qed.
+
+  #[global] Instance valid_ptr_sub_0 (p : ptr) ty :
+    HasSize ty ->
+    Observe (valid_ptr (p ,, o_sub σ ty 0)) (valid_ptr p).
+  Proof. intros. rewrite o_sub_0 // offset_ptr_id. refine _. Qed.
+  #[global] Instance type_ptr_sub_0 (p : ptr) ty :
+    HasSize ty ->
+    Observe (valid_ptr (p ,, o_sub σ ty 0)) (type_ptr ty p).
+  Proof.
+    intros. by rewrite type_ptr_valid; apply valid_ptr_sub_0.
+  Qed.
+  #[global] Instance type_ptr_valid_ptr_next (p : ptr) ty (m n : Z) :
+    (m = n + 1)%Z ->
+    Observe (valid_ptr (p ,, o_sub σ ty m)) (type_ptr ty (p ,, o_sub σ ty n)).
+  Proof.
+    intros; subst.
+    iIntros "X".
+    iDestruct (observe (valid_ptr (p ,, o_sub _ _ _ ,, o_sub _ _ _)) with "X") as "z".
+    apply observe_type_ptr_valid_plus_one. refine _.
+    by rewrite o_sub_sub.
+  Qed.
+
+  Lemma same_alloc_refl p : valid_ptr p ⊢ [| same_alloc p p |].
+  Proof.
+    rewrite valid_ptr_alloc_id same_alloc_iff. iIntros "!%". case; naive_solver.
+  Qed.
+
+  Lemma live_has_alloc_id p :
+    live_ptr p ⊢ ∃ aid, [| ptr_alloc_id p = Some aid |] ∗ live_alloc_id aid.
+  Proof. rewrite /live_ptr; iIntros. case: (ptr_alloc_id p) => /= [aid|]; eauto. Qed.
+
+  #[global] Instance struct_padding_as_fractional p cls : AsCFractional0 (struct_padding p cls).
+  Proof. solve_as_cfrac. Qed.
+  #[global] Instance struct_padding_valid_observe p q cls : Observe (strict_valid_ptr p) (struct_padding p cls q).
+  Proof. rewrite -type_ptr_strict_valid; apply _. Qed.
+  #[global] Instance struct_paddingR_valid_observe p q cls : Observe (valid_ptr p) (struct_padding p cls q).
+  Proof. rewrite -strict_valid_valid; apply _. Qed.
+
+  #[global] Instance union_padding_as_fractional p cls : AsCFractional1 (union_padding p cls).
+  Proof. solve_as_cfrac. Qed.
+
+  #[global] Instance union_padding_strict_valid_observe p q cls i : Observe (strict_valid_ptr p) (union_padding p cls q i).
+  Proof. rewrite -type_ptr_strict_valid; apply _. Qed.
+  #[global] Instance union_padding_valid_observe p q cls i : Observe (valid_ptr p) (union_padding p cls q i).
+  Proof. rewrite -strict_valid_valid; apply _. Qed.
+
+End with_cpp.
+
+Section has_type.
+  Context `{cpp_logic}.
+
+  (** [has_type] *)
+
+  #[global] Instance: Params (@has_type) 3 := {}.
+  #[global] Instance has_type_proper :
+    Proper (genv_eq ==> eq ==> eq ==> (≡)) (@has_type _ _ _).
+  Proof. intros ?? Heq ??? ???; split'; apply has_type_mono => //; apply Heq. Qed.
+
+  #[global] Instance has_type_flip_mono :
+    Proper (flip genv_leq ==> eq ==> eq ==> flip bi_entails) (@has_type _ _ _).
+  Proof. by move=> ??+ ??-> ??-> => ->. Qed.
+
+  #[global] Instance has_type_knowledge {σ} : Knowledge2 has_type_or_undef.
+  Proof. rewrite has_type_or_undef_unfold; split; apply _. Qed.
+  #[global] Instance has_type_timeless {σ} : Timeless2 has_type_or_undef.
+  Proof. rewrite has_type_or_undef_unfold; apply _. Qed.
+
+  Lemma has_type_nonptr {σ} v ty :
+    nonptr_prim_type ty ->
+    has_type v ty -|- [| has_type_prop v ty |].
+  Proof.
+    intros. split'.
+    - by rewrite -has_type_has_type_prop.
+    - by rewrite -has_type_prop_has_type_noptr.
+  Qed.
+
+  Lemma has_type_qual_iff {σ} t q x :
+    has_type x t -|- has_type x (Tqualified q t).
+  Proof.
+    by rewrite (has_type_erase_qualifiers t)
+      (has_type_erase_qualifiers (Tqualified _ _)).
+  Qed.
+
+  Lemma has_type_drop_qualifiers {σ} v ty :
+    has_type v ty -|- has_type v (drop_qualifiers ty).
+  Proof.
+    rewrite (has_type_erase_qualifiers (drop_qualifiers _)) erase_drop_qualifiers.
+    by rewrite -has_type_erase_qualifiers.
+  Qed.
+
+  Lemma has_type_val_related {σ} ty v1 v2 :
+    val_related ty v1 v2 ->
+    has_type v1 ty -|- has_type v2 ty.
+  Proof.
+    induction 1.
+    { done. }
+    { by rewrite -!has_type_qual_iff. }
+    all: by rewrite !has_type_nonptr ?has_type_prop_raw_bytes_of_val.
+  Qed.
+
+  (** [has_type_or_undef] *)
+
+  Definition is_undef (v : val) : bool :=
+    if v is Vundef then true else false.
+
+  #[global] Instance: Params (@has_type_or_undef) 3 := {}.
+  #[global] Instance has_type_or_undef_proper :
+    Proper (genv_eq ==> eq ==> eq ==> (≡)) (@has_type_or_undef _ _ _).
+  Proof. rewrite has_type_or_undef_unfold; solve_proper. Qed.
+  #[global] Instance has_type_or_undef_mono :
+    Proper (genv_leq ==> eq ==> eq ==> (⊢)) (@has_type_or_undef _ _ _).
+  Proof. rewrite has_type_or_undef_unfold; solve_proper. Qed.
+
+  Lemma has_type_or_undef_undef {σ} t : |-- has_type_or_undef Vundef t.
+  Proof. rewrite has_type_or_undef_unfold. by iRight. Qed.
+
+  Lemma has_type_or_undef_nonundef {σ} t v :
+    ~~ is_undef v -> has_type_or_undef v t -|- has_type v t.
+  Proof.
+    intros. rewrite has_type_or_undef_unfold. split'.
+    - iIntros "[$ | %]". by destruct v.
+    - iIntros "?". by iLeft.
+  Qed.
+
+  Lemma has_type_or_undef_qual_iff {σ} t q v :
+    has_type_or_undef v t -|- has_type_or_undef v (Tqualified q t).
+  Proof.
+    by rewrite !has_type_or_undef_unfold -!has_type_qual_iff.
+  Qed.
+
+  Lemma has_type_or_undef_val_related {σ} ty v1 v2 :
+    val_related ty v1 v2 ->
+    has_type_or_undef v1 ty |-- has_type_or_undef v2 ty.
+  Proof.
+    induction 1.
+    { done. }
+    { by rewrite -!has_type_or_undef_qual_iff. }
+    all: rewrite !has_type_or_undef_nonundef//.
+    all: by rewrite !has_type_nonptr// has_type_prop_raw_bytes_of_val.
+  Qed.
+End has_type. *)
+
+#[global] Notation "'validP<' ty > v" := (has_type v ty%cpp_type)
+  (at level 30, ty at level 20, v at level 1, format "validP< ty >  v") : bi_scope.
